WIP

theories/prelude/smallstr.v
@@ -15,6 +15,8 @@ Require Coq.Numbers.BinNums.
 
 Import Uint63 PArray.
 
+#[global] Declare Scope smallstr_scope.
+#[global] Delimit Scope smallstr_scope with smallstr.
 
 Module SmallStr.
 (* Encoding of strings using packed bits
@@ -25,6 +27,20 @@ Module SmallStr.
 #[projections(primitive=yes)]
 Record t : Set := Smallstr { smallstr_bytes : array Uint63.int }.
 #[global] Notation smallstr := t.
+#[global] Bind Scope smallstr_scope with t.
+
+#[program]
+Definition eq_dec s1 s2 : Decision (s1 = s2) :=
+  match PArray.eq_dec s1.(smallstr_bytes) s2.(smallstr_bytes) with
+  | left _ => left _
+  | right _ => right _
+  end.
+Next Obligation. intros [] []. simpl. now intros ->. Qed.
+Next Obligation. intros [] []. simpl. intros H E. apply H. now injection E. Qed.
+
+Definition eqb (s1 s2 : smallstr) := match eq_dec s1 s2 with left _ => true | _ => false end.
+
+#[global] Instance smallstr_eqdec : EqDecision smallstr := eq_dec.
 
 Definition bit (n : Uint63.int) (b : bool) : Uint63.int :=
   if b
@@ -47,20 +63,320 @@ Section with_notation.
     | xO p => pos_to_int p (Uint63.lsl acc 1)
     end.
 
-  Search byte N.
   Definition to_int (a : Byte.byte) : Uint63.int :=
     of_Z (BinIntDef.Z.of_N (to_N a)).
 
   #[local]
-  Definition int_to_nat (i : int) : nat := BinIntDef.Z.to_nat (to_Z i).
+  Definition int_to_nat' (i : int) : nat := BinIntDef.Z.to_nat (to_Z i).
+
+  Definition some_nats_limit := 255%uint63.
+  Definition some_nats :=
+    Eval vm_compute in
+    let a := PArray.make 255 0 in
+    let go :=
+      fix go n i a :=
+        match n with
+        | 0 => a
+        | S n => go n (i+1)%uint63 (PArray.set a i (int_to_nat' i))
+        end
+    in
+    go (int_to_nat' some_nats_limit) 0%uint63 a.
+
+  Definition int_to_nat i :=
+    Eval lazy [some_nats] in
+    if Uint63.ltb i some_nats_limit then some_nats.[i] else int_to_nat' i.
+
   #[local]
-  Definition int_to_byte (i : int) : Byte.byte :=
+  Definition int_to_byte' (i : int) : Byte.byte :=
     match of_N (BinIntDef.Z.to_N (to_Z i)) with
     | None => x00
     | Some x => x
     end.
 
+  Definition all_bytes : array byte :=
+    Eval vm_compute in
+    let a := PArray.make 255 x00 in
+    let go :=
+      fix go n i a :=
+        match n with
+        | 0 => a
+        | S n => go n (i+1)%uint63 (PArray.set a i (int_to_byte' i))
+        end
+    in
+    go 255 0%uint63 a.
+
+  Definition int_to_byte i := all_bytes.[i].
+
 End with_notation.
+
+Definition to_bits : forall (i : int), list nat :=
+  let go := fix go n acc i :=
+      match n with
+      | 0 => acc
+      | S n => go n (int_to_nat (i land 1) :: acc)%uint63 (i >> 1)%uint63
+      end
+  in
+  go 63 [].
+
+Eval lazy in to_bits (255<<48)%uint63.
+
+Definition max_val := Eval cbv in (max_int >> 7)%uint63.
+Definition zero_mask sh := ((255 << (sh * 8)) lxor max_val)%uint63.
+(* Mask out n many characters from the suffix *)
+Definition zero_masks n := (max_val >> (n * 8))%uint63.
+
+Eval lazy in to_bits (zero_masks 6).
+
+Definition len s := let '{|smallstr_bytes := a|} := s in get a 0%uint63.
+
+Definition position (i : Uint63.int) : Uint63.int * Uint63.int :=
+  let (q,r) := Uint63.diveucl i 7 in
+  (* index 0 is the string length *)
+  (q+1, r)%uint63.
+
+Definition div_up (i1 i2 : int) :=
+  let (q,r) := diveucl i1 i2 in
+  if Uint63.eqb r 0 then q else (q + 1)%uint63.
+
+
+(* "abcd" is [4; "d" << 24 + "c" << 16 + "b" << 8 + "a" ].
+   This violates prefix order
+ *)
+Module BigEndian.
+
+Fixpoint next_string_big (acc : Uint63.int) (n : nat) (s : list Byte.byte) sh : Uint63.int * list Byte.byte :=
+  match n , s with
+  | S n , List.cons b s =>
+    next_string_big (Uint63.lor acc (to_int b << sh)%uint63) n s (sh + 8)%uint63
+  | _ , nil => (acc, s)
+  | 0%nat , s => (acc, s)
+  end.
+
+Definition fill :=
+  Eval lazy [next_string_big Uint63.add] in
+  fix fill n s i arr {struct n} :=
+  match s with
+  | [] => arr
+  | _ =>
+      match n with
+      | 0 => arr
+      | S n =>
+          let (v,s) := next_string_big 0 7 s 0 in
+          fill n s (i + 1)%uint63 (set arr i v)
+      end
+  end.
+
+Definition parse (s : list byte) : smallstr :=
+  let len_nat := List.length s in
+  let len := nat_to_int len_nat 0 in
+  (* 1 uint63 for the string length + ceil(n/7) uint63 for the bytes *)
+  let arrlen := (1 + (div_up len 7))%uint63 in
+  let arr := PArray.make arrlen 0%uint63 in
+  let arr := PArray.set arr 0 len in
+  Smallstr (fill len_nat s 1%int63 arr).
+
+Eval lazy in
+  let s := parse [x00; x00; x00; x00; x00; x00; x00; x61; x62; x63; x64; x65; x66] in
+  s.
+
+
+Fixpoint read_bytes (n : nat) (i : int) (acc : list byte) : list byte :=
+  match n with
+  | 0 => acc
+  | S n =>
+      let b := (i land 255)%uint63 in
+      let i := (i >> 8)%uint63 in
+      (int_to_byte' b) :: read_bytes n i acc
+  end.
+
+Definition print_aux_new a from len : list byte :=
+Eval cbn beta fix match delta [read_bytes] in
+  let fuel := int_to_nat (div_up len 7) in
+  let todo := (from+len)%uint63 in
+  let last := div_up todo 7 in
+  let go :=
+    fix go n pos ind todo acc {struct n} :=
+      match n with
+      | 0 => acc
+      | S n =>
+          let bucket := PArray.get a pos in
+          let bucketlen := (Uint63.mod ind 7)%uint63 in
+          let bucketlen := if Uint63.eqb bucketlen 0 then 7%uint63 else bucketlen in
+          let '(bucketlen, bucket) :=
+            if Uint63.ltb todo bucketlen then
+              (todo, (bucket >> ((7-todo) * 8))%uint63)
+            else
+              (bucketlen, bucket)
+          in
+          let bucketlen_nat := int_to_nat bucketlen in
+          let ind := (ind - bucketlen)%uint63 in
+          let todo := (todo - bucketlen)%uint63 in
+          let pos := (pos - 1)%uint63 in
+          go n pos ind todo (read_bytes bucketlen_nat bucket acc)
+      end
+  in
+  go fuel last todo len [].
+
+Definition print_aux a from len : list byte :=
+Eval cbn beta fix match delta [read_bytes] in
+  let fuel := int_to_nat len in
+  let last := div_up (from+len) 7 in
+  let go :=
+    fix go n pos ind todo acc {struct n} :=
+      match n with
+      | 0 => acc
+      | S n as m =>
+          let bucket := PArray.get a pos in
+          (* let bytes := read_bytes bucketlen bucket acc in *)
+          let pos := (pos - 1)%uint63 in
+          let bucketlen := (Uint63.mod ind 7)%uint63 in
+          let bucketlen_nat := int_to_nat bucketlen in
+          let ind := (ind - bucketlen)%uint63 in
+          let todo := (todo - bucketlen)%uint63 in
+          match bucketlen_nat, n with
+          | 0, S (S (S (S (S (S n))))) => go n pos ind todo (read_bytes 7 bucket acc)
+          | 6,   (S (S (S (S (S n))))) => go n pos ind todo (read_bytes 6 bucket acc)
+          | 5,   (  (S (S (S (S n))))) => go n pos ind todo (read_bytes 5 bucket acc)
+          | 4,   (  (  (S (S (S n))))) => go n pos ind todo (read_bytes 4 bucket acc)
+          | 3,   (  (  (  (S (S n))))) => go n pos ind todo (read_bytes 3 bucket acc)
+          | 2,   (  (  (  (  (S n))))) => go n pos ind todo (read_bytes 2 bucket acc)
+          | 1,   (  (  (  (  (  n))))) => go n pos ind todo (read_bytes 1 bucket acc)
+          | _, _ =>
+              let bucketlen := if Uint63.eqb bucketlen 0 then 7%uint63 else bucketlen in
+              let '(skip, bucketlen, bucket) :=
+                if Uint63.ltb todo bucketlen then
+                  (int_to_nat (7-todo)%uint63, todo, (bucket >> ((7-todo) * 8))%uint63)
+                else
+                  (0, bucketlen, bucket)
+              in
+              read_bytes bucketlen_nat bucket acc
+          end
+      end
+  in
+  go fuel last (from+len)%uint63 len [].
+
+
+Definition print_new s : list byte :=
+Eval cbn beta fix match delta [read_bytes] in
+  let a := s.(smallstr_bytes) in
+  let len := get a 0%uint63 in
+  let len_nat := int_to_nat len in
+  let last := div_up len 7 in
+  let go :=
+    fix go n pos bucketlen acc {struct n} :=
+      match n with
+      | 0 => acc
+      | S n as m =>
+          let bucket := PArray.get a pos in
+          (* let bytes := read_bytes bucketlen bucket acc in *)
+          go n (pos - 1)%uint63 7 (read_bytes bucketlen bucket acc)
+      end
+  in
+  let bucketlen :=
+    match (int_to_nat (Uint63.mod len 7)) with
+    | 0 => 7
+    | _ as b => b
+    end
+  in
+  go (int_to_nat last) last bucketlen [].
+
+Definition print s : list byte :=
+Eval cbn beta fix match delta [read_bytes] in
+  let a := s.(smallstr_bytes) in
+  let len := get a 0%uint63 in
+  let len_nat := int_to_nat len in
+  let last := div_up len 7 in
+  let go :=
+    fix go n pos bucketlen acc {struct n} :=
+      match n with
+      | 0 => acc
+      | S n as m =>
+          let bucket := PArray.get a pos in
+          match bucketlen, n with
+          | 0, S (S (S (S (S (S n))))) => go n (pos - 1)%uint63 0 (read_bytes 7 bucket acc)
+          | 6,   (S (S (S (S (S n))))) => go n (pos - 1)%uint63 0 (read_bytes 6 bucket acc)
+          | 5,   (  (S (S (S (S n))))) => go n (pos - 1)%uint63 0 (read_bytes 5 bucket acc)
+          | 4,   (  (  (S (S (S n))))) => go n (pos - 1)%uint63 0 (read_bytes 4 bucket acc)
+          | 3,   (  (  (  (S (S n))))) => go n (pos - 1)%uint63 0 (read_bytes 3 bucket acc)
+          | 2,   (  (  (  (  (S n))))) => go n (pos - 1)%uint63 0 (read_bytes 2 bucket acc)
+          | 1,   (  (  (  (  (  n))))) => go n (pos - 1)%uint63 0 (read_bytes 1 bucket acc)
+          | _, _ => read_bytes bucketlen bucket acc
+          end
+      end
+  in
+  go len_nat last (int_to_nat (Uint63.mod len 7)) [].
+
+Definition print2 s : list byte :=
+Eval lazy beta fix match delta [print_aux Uint63.add] in
+  let a := s.(smallstr_bytes) in
+  let len := get a 0%uint63 in
+  print_aux a 0 len.
+
+Definition print2_new s : list byte :=
+Eval lazy beta fix match delta [print_aux_new] in
+  let a := s.(smallstr_bytes) in
+  let len := get a 0%uint63 in
+  print_aux_new a 0 len.
+
+(* Eval lazy in print_aux_new (parse [x61;x62;x63;x64;x65;x66;x67;x68]).(smallstr_bytes) 0 8. *)
+
+
+Instructions Eval lazy in
+  let l := repeat x61 1000 in
+  let s := parse l in
+  List.length (print_new s).
+Instructions Eval vm_compute in
+  let l := repeat x61 1000 in
+  let s := parse l in
+  List.length (print_new s).
+
+Instructions Eval lazy in
+  let l := repeat x61 1000 in
+  let s := parse l in
+  List.length (print2_new s).
+Instructions Eval vm_compute in
+  let l := repeat x61 1000 in
+  let s := parse l in
+  List.length (print2_new s).
+(* 49244932 *)
+(* 56597152 *)
+
+Instructions Eval lazy in
+  let l := repeat x61 1000 in
+  let s := parse l in
+  List.length (print2 s).
+Instructions Eval vm_compute in
+  let l := repeat x61 1000 in
+  let s := parse l in
+  List.length (print2 s).
+(* 159097997 *)
+(*  59796203 *)
+
+
+Instructions Eval lazy in
+  let l := repeat x61 1000 in
+  let s := parse l in
+  List.length (print s).
+Instructions Eval vm_compute in
+  let l := repeat x61 1000 in
+  let s := parse l in
+  List.length (print s).
+(* 55441262 *)
+(* 56904102 *)
+
+
+Instructions Eval lazy in
+  let l := repeat x61 10000 in
+  let s := parse l in
+  PArray.get s.(smallstr_bytes) 0.
+Instructions Eval vm_compute in
+  let l := repeat x61 10000 in
+  let s := parse l in
+  PArray.get s.(smallstr_bytes) 0.
+(* 500850420 *)
+(*  26930178 *)
+
+
 
 #[local]
 Fixpoint next_string (acc : Uint63.int) (n : nat) (s : list Byte.byte) : Uint63.int * list Byte.byte :=
@@ -71,7 +387,8 @@ Fixpoint next_string (acc : Uint63.int) (n : nat) (s : list Byte.byte) : Uint63.
   | 0%nat , s => (acc, s)
   end.
 
-Definition parse (s : list Byte.byte) : smallstr :=
+
+Definition parse' (s : list Byte.byte) : smallstr :=
   let n := List.length s in
   let len := nat_to_int n 0 in
   let empty := make (((6+7) + len) / 7)%uint63 0%uint63 in
@@ -86,7 +403,18 @@ Definition parse (s : list Byte.byte) : smallstr :=
            end
      end) 1%int63 n s arr).
 
-Definition print (s : smallstr) : list Byte.byte :=
+Instructions Eval lazy in
+  let l := repeat x61 10000 in
+  let s := parse' l in
+  PArray.get s.(smallstr_bytes) 0.
+Instructions Eval vm_compute in
+  let l := repeat x61 10000 in
+  let s := parse' l in
+  PArray.get s.(smallstr_bytes) 0.
+(* 321613359 *)
+(*  26930178 *)
+
+Definition print' (s : smallstr) : list Byte.byte :=
   let s := s.(smallstr_bytes) in
   let len := get s 0%uint63 in
   let len_nat := int_to_nat len in
@@ -108,22 +436,453 @@ Definition print (s : smallstr) : list Byte.byte :=
        a :: go rest resti nexti nextr byte
      end)%uint63 len_nat len 2%uint63 (shift len) (get s 1).
 
+Instructions Eval lazy in
+  let l := repeat x61 1000 in
+  let s := parse' l in
+  List.length (print' s).
+Instructions Eval vm_compute in
+  let l := repeat x61 1000 in
+  let s := parse' l in
+  List.length (print' s).
+(* 67383816 *)
+(* 57238290 *)
+
+Eval cbv in (max_int >> (7 * 8))%uint63.
+Eval cbv in ((max_int << (5 * 8)) lor (max_int >> ((7 - 5 + 1) * 8)))%uint63.
+Eval cbv in (max_int land (1 << 8))%uint63.
+
+
+(* [set s i b] sets byte [i] to value [b] in string [s]. Returns [s] unchanged if [i] is bigger or equal to the [len s]. *)
+Definition set_byte s i (b : byte) :=
+  if (Uint63.leb (len s) i) then s
+  else
+    let '{|smallstr_bytes := a|} := s in
+    let (pos, sh) := position i in
+    let bucket := PArray.get a pos in
+    let bucket := ((bucket land zero_mask sh) lxor (to_int b << (sh * 8)))%uint63 in
+    let a := PArray.set a pos bucket in
+    {|smallstr_bytes := a|}.
+
+Fixpoint set_bytes s i (bs : list byte) :=
+  match bs with
+  | [] => s
+  | b :: bs =>
+      set_bytes (set_byte s i b) (i+1)%uint63 bs
+  end.
+
+(* [extend s n] extends [s] by [n] many zero bytes. *)
+Definition extend s (n : int) :=
+  if Uint63.eqb n 0 then s else
+  let '{|smallstr_bytes := a|} := s in
+  let slen := len s in
+  let (q, r) := diveucl slen 7 in
+  let cap := (7-r)%uint63 in
+  let total := (slen + n)%uint63 in
+  if Uint63.leb n cap then
+    {|smallstr_bytes := PArray.set a 0 total|}
+  else
+    let newlen := (1+div_up total 7)%uint63 in
+    let out := PArray.make newlen 0%uint63 in
+    (* TODO: [foldl_i] with offset to skip first item *)
+    let out := PArray.foldl_i (fun i v out => PArray.set out i v) a out in
+    (* fix length *)
+    let out := PArray.set out 0 total in
+    Smallstr out.
+
+(* [shrink s n] masks out all but the first [n] elements in [s].
+   Only allocates if [n] is smaller than the current length.
+ *)
+Definition shrink s (n : int) :=
+  let '{|smallstr_bytes := a|} := s in
+  let slen := len s in
+  if Uint63.leb slen n then
+    s (* we already no more than [n] elements *)
+  else
+    let last := div_up n 7 in
+    let newlen := (1+last)%uint63 in
+    let partial := (Uint63.mod n 7)%uint63 in
+    let out := PArray.make newlen 0%uint63 in
+    let out := PArray.foldl_i (fun i _ out => PArray.set out i (PArray.get a i)) out out in
+    let out := PArray.set out 0 n in
+    let out :=
+      if Uint63.eqb partial 0 then out else
+      PArray.set out last (PArray.get out last land zero_masks (7-partial))%uint63
+    in
+    Smallstr out.
+
+Definition append s1 s2 :=
+  let len2 := len s2 in
+  if Uint63.eqb len2 0 then s1 else
+  let len1 := len s1 in
+  if Uint63.eqb len2 0 then s2 else
+  (* let newlen := len1 + len2 in *)
+  (* let '{|smallstr_bytes := a1|} := s1 in *)
+  (* let '{|smallstr_bytes := a2|} := s2 in *)
+  let s3 := extend s1 len2 in
+  snd (List.fold_left (fun '(i,out) b => ((i+1)%uint63, set_byte out i b)) (print s2) (len1, s3)).
+
+Eval lazy in append (parse (repeat x61 5)) (parse (repeat x62 5)).
+Eval lazy in print (append (parse (repeat x61 5)) (parse (repeat x62 5))).
+
+(* [sub s start l] returns a new string that contains bytes [start .. start+l-1] of [s]. *)
+Definition sub s start l :=
+  let len := len s in
+  if Uint63.eqb start 0 && Uint63.eqb l len then s else
+  if Uint63.leb len start then Smallstr (PArray.make 1%uint63 0%uint63) else
+  let '{|smallstr_bytes := a|} := s in
+  let rem := (len-start)%uint63 in
+  let newlen := if Uint63.leb l rem then l else rem in
+  let last := div_up newlen 7 in
+  let newarrlen := (1+last)%uint63 in
+  let partial := (Uint63.mod newlen 7)%uint63 in
+  let out := PArray.make newarrlen 0%uint63 in
+  let out := PArray.foldl_i (fun i _ out => PArray.set out i (PArray.get a (i+start))) out out in
+  let out := PArray.set out 0 newlen in
+  let out :=
+    if Uint63.eqb partial 0 then out else
+    PArray.set out last (PArray.get out last land zero_masks (7-partial))%uint63
+  in
+  Smallstr out.
+
+Eval lazy in print (sub (parse ["a"; "b"; "c"; "d"]%byte) 0 4).
+
+End BigEndian.
+
+
+Fixpoint next_string (acc : Uint63.int) (n : nat) (s : list Byte.byte) : Uint63.int * list Byte.byte :=
+  match n , s with
+  | S n , List.cons b s =>
+    next_string (Uint63.lor (Uint63.lsl acc 8%int63) (to_int b)) n s
+  | _ , _ => (acc, s)
+  end.
+
+Definition fill :=
+  Eval lazy [next_string Uint63.add] in
+  fix fill n s i arr {struct n} :=
+  match s with
+  | [] => arr
+  | _ =>
+      match n with
+      | 0 => arr
+      | S n =>
+          let (v,s) := next_string 0 7 s in
+          fill n s (i + 1)%uint63 (set arr i v)
+      end
+  end.
+
+Definition parse (s : list byte) : smallstr :=
+  let len_nat := List.length s in
+  let len := nat_to_int len_nat 0 in
+  (* 1 uint63 for the string length + ceil(n/7) uint63 for the bytes *)
+  let arrlen := (1 + (div_up len 7))%uint63 in
+  let arr := PArray.make arrlen 0%uint63 in
+  let arr := PArray.set arr 0 len in
+  Smallstr (fill len_nat s 1%int63 arr).
+
+Eval lazy in
+  let s := parse [x61; x62; x63; x64; x65] in
+  s.
+
+Eval lazy in
+  parse [x61; x62; x63; x64; x65].
+
+
+Fixpoint read_bytes (n : nat) (i : int) (acc : list byte) : list byte :=
+  match n with
+  | 0 => acc
+  | S n =>
+      let b := (i land 255)%uint63 in
+      let i := (i >> 8)%uint63 in
+      read_bytes n i (int_to_byte' b :: acc)
+  end.
+
+Definition print_aux_new a from len : list byte :=
+Eval cbn beta fix match delta [read_bytes] in
+  let fuel := int_to_nat (div_up len 7) in
+  let todo := (from+len)%uint63 in
+  let last := div_up todo 7 in
+  let go :=
+    fix go n pos ind todo acc {struct n} :=
+      match n with
+      | 0 => acc
+      | S n =>
+          let bucket := PArray.get a pos in
+          let bucketlen := (Uint63.mod ind 7)%uint63 in
+          let bucketlen := if Uint63.eqb bucketlen 0 then 7%uint63 else bucketlen in
+          let '(bucketlen, bucket) :=
+            if Uint63.ltb todo bucketlen then
+              (todo, (bucket >> ((7-todo) * 8))%uint63)
+            else
+              (bucketlen, bucket)
+          in
+          let bucketlen_nat := int_to_nat bucketlen in
+          let ind := (ind - bucketlen)%uint63 in
+          let todo := (todo - bucketlen)%uint63 in
+          let pos := (pos - 1)%uint63 in
+          go n pos ind todo (read_bytes bucketlen_nat bucket acc)
+      end
+  in
+  go fuel last todo len [].
+
+Definition print_aux a from len : list byte :=
+Eval cbn beta fix match delta [read_bytes] in
+  let fuel := int_to_nat len in
+  let last := div_up (from+len) 7 in
+  let go :=
+    fix go n pos ind todo acc {struct n} :=
+      match n with
+      | 0 => acc
+      | S n as m =>
+          let bucket := PArray.get a pos in
+          (* let bytes := read_bytes bucketlen bucket acc in *)
+          let pos := (pos - 1)%uint63 in
+          let bucketlen := (Uint63.mod ind 7)%uint63 in
+          let bucketlen_nat := int_to_nat bucketlen in
+          let ind := (ind - bucketlen)%uint63 in
+          let todo := (todo - bucketlen)%uint63 in
+          match bucketlen_nat, n with
+          | 0, S (S (S (S (S (S n))))) => go n pos ind todo (read_bytes 7 bucket acc)
+          | 6,   (S (S (S (S (S n))))) => go n pos ind todo (read_bytes 6 bucket acc)
+          | 5,   (  (S (S (S (S n))))) => go n pos ind todo (read_bytes 5 bucket acc)
+          | 4,   (  (  (S (S (S n))))) => go n pos ind todo (read_bytes 4 bucket acc)
+          | 3,   (  (  (  (S (S n))))) => go n pos ind todo (read_bytes 3 bucket acc)
+          | 2,   (  (  (  (  (S n))))) => go n pos ind todo (read_bytes 2 bucket acc)
+          | 1,   (  (  (  (  (  n))))) => go n pos ind todo (read_bytes 1 bucket acc)
+          | _, _ =>
+              let bucketlen := if Uint63.eqb bucketlen 0 then 7%uint63 else bucketlen in
+              let '(skip, bucketlen, bucket) :=
+                if Uint63.ltb todo bucketlen then
+                  (int_to_nat (7-todo)%uint63, todo, (bucket >> ((7-todo) * 8))%uint63)
+                else
+                  (0, bucketlen, bucket)
+              in
+              read_bytes bucketlen_nat bucket acc
+          end
+      end
+  in
+  go fuel last (from+len)%uint63 len [].
+
+
+Definition print_new s : list byte :=
+Eval cbn beta fix match delta [read_bytes] in
+  let a := s.(smallstr_bytes) in
+  let len := get a 0%uint63 in
+  let len_nat := int_to_nat len in
+  let last := div_up len 7 in
+  let go :=
+    fix go n pos bucketlen acc {struct n} :=
+      match n with
+      | 0 => acc
+      | S n as m =>
+          let bucket := PArray.get a pos in
+          (* let bytes := read_bytes bucketlen bucket acc in *)
+          go n (pos - 1)%uint63 7 (read_bytes bucketlen bucket acc)
+      end
+  in
+  let bucketlen :=
+    match (int_to_nat (Uint63.mod len 7)) with
+    | 0 => 7
+    | _ as b => b
+    end
+  in
+  go (int_to_nat last) last bucketlen [].
+
+Definition print s : list byte :=
+Eval cbn beta fix match delta [read_bytes] in
+  let a := s.(smallstr_bytes) in
+  let len := get a 0%uint63 in
+  let len_nat := int_to_nat len in
+  let last := div_up len 7 in
+  let go :=
+    fix go n pos bucketlen acc {struct n} :=
+      match n with
+      | 0 => acc
+      | S n as m =>
+          let bucket := PArray.get a pos in
+          match bucketlen, n with
+          | 0, S (S (S (S (S (S n))))) => go n (pos - 1)%uint63 0 (read_bytes 7 bucket acc)
+          | 6,   (S (S (S (S (S n))))) => go n (pos - 1)%uint63 0 (read_bytes 6 bucket acc)
+          | 5,   (  (S (S (S (S n))))) => go n (pos - 1)%uint63 0 (read_bytes 5 bucket acc)
+          | 4,   (  (  (S (S (S n))))) => go n (pos - 1)%uint63 0 (read_bytes 4 bucket acc)
+          | 3,   (  (  (  (S (S n))))) => go n (pos - 1)%uint63 0 (read_bytes 3 bucket acc)
+          | 2,   (  (  (  (  (S n))))) => go n (pos - 1)%uint63 0 (read_bytes 2 bucket acc)
+          | 1,   (  (  (  (  (  n))))) => go n (pos - 1)%uint63 0 (read_bytes 1 bucket acc)
+          | _, _ => read_bytes bucketlen bucket acc
+          end
+      end
+  in
+  go len_nat last (int_to_nat (Uint63.mod len 7)) [].
+
+Definition print2 s : list byte :=
+Eval lazy beta fix match delta [print_aux Uint63.add] in
+  let a := s.(smallstr_bytes) in
+  let len := get a 0%uint63 in
+  print_aux a 0 len.
+
+Definition print2_new s : list byte :=
+Eval lazy beta fix match delta [print_aux_new] in
+  let a := s.(smallstr_bytes) in
+  let len := get a 0%uint63 in
+  print_aux_new a 0 len.
+
+(* Eval lazy in print_aux_new (parse [x61;x62;x63;x64;x65;x66;x67;x68]).(smallstr_bytes) 0 8. *)
+
+
+Instructions Eval lazy in
+  let l := repeat x61 1000 in
+  let s := parse l in
+  List.length (print_new s).
+Instructions Eval vm_compute in
+  let l := repeat x61 1000 in
+  let s := parse l in
+  List.length (print_new s).
+
+Instructions Eval lazy in
+  let l := repeat x61 1000 in
+  let s := parse l in
+  List.length (print2_new s).
+Instructions Eval vm_compute in
+  let l := repeat x61 1000 in
+  let s := parse l in
+  List.length (print2_new s).
+(* 49244932 *)
+(* 56597152 *)
+
+Instructions Eval lazy in
+  let l := repeat x61 1000 in
+  let s := parse l in
+  List.length (print2 s).
+Instructions Eval vm_compute in
+  let l := repeat x61 1000 in
+  let s := parse l in
+  List.length (print2 s).
+(* 159097997 *)
+(*  59796203 *)
+
+
+Instructions Eval lazy in
+  let l := repeat x61 1000 in
+  let s := parse l in
+  List.length (print s).
+Instructions Eval vm_compute in
+  let l := repeat x61 1000 in
+  let s := parse l in
+  List.length (print s).
+(* 55441262 *)
+(* 56904102 *)
+
+
+Instructions Eval lazy in
+  let l := repeat x61 10000 in
+  let s := parse l in
+  PArray.get s.(smallstr_bytes) 0.
+Instructions Eval vm_compute in
+  let l := repeat x61 10000 in
+  let s := parse l in
+  PArray.get s.(smallstr_bytes) 0.
+(* 500850420 *)
+(*  26930178 *)
+
+
+
+
+(* [set s i b] sets byte [i] to value [b] in string [s]. Returns [s] unchanged if [i] is bigger or equal to the [len s]. *)
+Definition set_byte s i (b : byte) :=
+  if (Uint63.leb (len s) i) then s
+  else
+    let '{|smallstr_bytes := a|} := s in
+    let (pos, sh) := position i in
+    let bucket := PArray.get a pos in
+    let bucket := ((bucket land zero_mask sh) lxor (to_int b << (sh * 8)))%uint63 in
+    let a := PArray.set a pos bucket in
+    {|smallstr_bytes := a|}.
+
+Fixpoint set_bytes s i (bs : list byte) :=
+  match bs with
+  | [] => s
+  | b :: bs =>
+      set_bytes (set_byte s i b) (i+1)%uint63 bs
+  end.
+
+(* [extend s n] extends [s] by [n] many zero bytes. *)
+Definition extend s (n : int) :=
+  if Uint63.eqb n 0 then s else
+  let '{|smallstr_bytes := a|} := s in
+  let slen := len s in
+  let (q, r) := diveucl slen 7 in
+  let cap := (7-r)%uint63 in
+  let total := (slen + n)%uint63 in
+  if Uint63.leb n cap then
+    {|smallstr_bytes := PArray.set a 0 total|}
+  else
+    let newlen := (1+div_up total 7)%uint63 in
+    let out := PArray.make newlen 0%uint63 in
+    (* TODO: [foldl_i] with offset to skip first item *)
+    let out := PArray.foldl_i (fun i v out => PArray.set out i v) a out in
+    (* fix length *)
+    let out := PArray.set out 0 total in
+    Smallstr out.
+
+(* [shrink s n] masks out all but the first [n] elements in [s].
+   Only allocates if [n] is smaller than the current length.
+ *)
+Definition shrink s (n : int) :=
+  let '{|smallstr_bytes := a|} := s in
+  let slen := len s in
+  if Uint63.leb slen n then
+    s (* we already no more than [n] elements *)
+  else
+    let last := div_up n 7 in
+    let newlen := (1+last)%uint63 in
+    let partial := (Uint63.mod n 7)%uint63 in
+    let out := PArray.make newlen 0%uint63 in
+    let out := PArray.foldl_i (fun i _ out => PArray.set out i (PArray.get a i)) out out in
+    let out := PArray.set out 0 n in
+    let out :=
+      if Uint63.eqb partial 0 then out else
+      PArray.set out last (PArray.get out last land zero_masks (7-partial))%uint63
+    in
+    Smallstr out.
+
+Definition append s1 s2 :=
+  let len2 := len s2 in
+  if Uint63.eqb len2 0 then s1 else
+  let len1 := len s1 in
+  if Uint63.eqb len2 0 then s2 else
+  (* let newlen := len1 + len2 in *)
+  (* let '{|smallstr_bytes := a1|} := s1 in *)
+  (* let '{|smallstr_bytes := a2|} := s2 in *)
+  let s3 := extend s1 len2 in
+  snd (List.fold_left (fun '(i,out) b => ((i+1)%uint63, set_byte out i b)) (print s2) (len1, s3)).
+
+Eval lazy in append (parse (repeat x61 5)) (parse (repeat x62 5)).
+Eval lazy in print (append (parse (repeat x61 5)) (parse (repeat x62 5))).
+
+(* [sub s start l] returns a new string that contains bytes [start .. start+l-1] of [s]. *)
+Definition sub s start l :=
+  let len := len s in
+  if Uint63.eqb start 0 && Uint63.eqb l len then s else
+  if Uint63.leb len start then Smallstr (PArray.make 1%uint63 0%uint63) else
+  let '{|smallstr_bytes := a|} := s in
+  let rem := (len-start)%uint63 in
+  let newlen := if Uint63.leb l rem then l else rem in
+  let last := div_up newlen 7 in
+  let newarrlen := (1+last)%uint63 in
+  let out := PArray.make newarrlen 0%uint63 in
+  let bytes := print_aux_new a start l in
+  let out := Smallstr (PArray.set out 0 newlen) in
+  let out := List.fold_left (fun '(i, out) b => ((i+1)%uint63, set_byte out i b)) bytes (0%uint63,out) in
+  out.2.
+
+Eval lazy in print_aux_new (parse ["a"; "b"; "c"; "d"]%byte).(smallstr_bytes) 1 3.
+
+Eval lazy in print (sub (parse ["a"; "b"; "c"; "d"]%byte) 1 4).
+
+
 Import BinInt.
 
 
-#[program]
-Definition eq_dec s1 s2 : Decision (s1 = s2) :=
-  match PArray.eq_dec s1.(smallstr_bytes) s2.(smallstr_bytes) with
-  | left _ => left _
-  | right _ => right _
-  end.
-Next Obligation. intros [] []. simpl. now intros ->. Qed.
-Next Obligation. intros [] []. simpl. intros H E. apply H. now injection E. Qed.
-
-Definition eqb (s1 s2 : smallstr) := match eq_dec s1 s2 with left _ => true | _ => false end.
-
-#[global] Instance smallstr_eqdec : EqDecision smallstr := eq_dec.
-
+#[global] String Notation SmallStr.smallstr SmallStr.parse SmallStr.print_new : smallstr_scope.
 
 Definition compare s1 s2 :=
   (PArray.compare (cmp:=Uint63.compare) s1.(smallstr_bytes) s2.(smallstr_bytes)).
@@ -221,10 +980,12 @@ Next Obligation.
 Qed.
 End SmallStr.
 
-#[global] Declare Scope smallstr_scope.
-#[global] Delimit Scope smallstr_scope with smallstr.
-#[global] Bind Scope smallstr_scope with SmallStr.smallstr.
+#[global] Bind Scope smallstr_scope with SmallStr.t.
 #[global] String Notation SmallStr.smallstr SmallStr.parse SmallStr.print : smallstr_scope.
+
+Eval cbv in "ab"%smallstr.(SmallStr.smallstr_bytes).
+
+Eval cbv in SmallStr.set_byte "test"%smallstr 3 x61.
 
 (* Unset Printing Notations. *)
 Eval lazy in SmallStr.smallstr_bytes "abcdefghi000000adkfjadsfkjasdfkjasd;fkljads;fkjladsfadsfadsfadsf".
@@ -248,6 +1009,7 @@ Module Type TEST.
   Succeed Example _1 : sanity "abcd" := I.
   Succeed Example _1 : sanity "abcde" := I.
   Succeed Example _1 : sanity "abcdef" := I.
+  Succeed Example _1 : sanity "abcdefg" := I.
   Succeed Example _1 : sanity "abcdefg" := I.
   Succeed Example _1 : sanity "abcdefgh" := I.
   Succeed Example _1 : sanity "abcdefghi" := I.
